\documentclass[journal,12pt,twocolumn]{IEEEtran}
%
\usepackage{setspace}
\usepackage{gensymb}
\usepackage{xcolor}
\usepackage{caption}
%\usepackage{subcaption}
%\doublespacing
\singlespacing

%\usepackage{graphicx}
%\usepackage{amssymb}
%\usepackage{relsize}
\usepackage[cmex10]{amsmath}
\usepackage{mathtools}
%\usepackage{amsthm}
%\interdisplaylinepenalty=2500
%\savesymbol{iint}
%\usepackage{txfonts}
%\restoresymbol{TXF}{iint}
%\usepackage{wasysym}
\usepackage{hyperref}
\usepackage{amsthm}
\usepackage{mathrsfs}
\usepackage{txfonts}
\usepackage{stfloats}
\usepackage{cite}
\usepackage{cases}
\usepackage{subfig}
%\usepackage{xtab}
\usepackage{longtable}
\usepackage{multirow}
%\usepackage{algorithm}
%\usepackage{algpseudocode}
%\usepackage{enumerate}
\usepackage{enumitem}
\usepackage{mathtools}
%\usepackage{iithtlc}
%\usepackage[framemethod=tikz]{mdframed}
\usepackage{listings}
\let\vec\mathbf


%\usepackage{stmaryrd}


%\usepackage{wasysym}
%\newcounter{MYtempeqncnt}
\DeclareMathOperator*{\Res}{Res}
%\renewcommand{\baselinestretch}{2}
\renewcommand\thesection{\arabic{section}}
\renewcommand\thesubsection{\thesection.\arabic{subsection}}
\renewcommand\thesubsubsection{\thesubsection.\arabic{subsubsection}}

\renewcommand\thesectiondis{\arabic{section}}
\renewcommand\thesubsectiondis{\thesectiondis.\arabic{subsection}}
\renewcommand\thesubsubsectiondis{\thesubsectiondis.\arabic{subsubsection}}

%\renewcommand{\labelenumi}{\textbf{\theenumi}}
%\renewcommand{\theenumi}{P.\arabic{enumi}}

% correct bad hyphenation here
\hyphenation{op-tical net-works semi-conduc-tor}

\lstset{
	language=Python,
	frame=single, 
	breaklines=true,
	columns=fullflexible
}



\begin{document}
	%
	
	\theoremstyle{definition}
	\newtheorem{theorem}{Theorem}[section]
	\newtheorem{problem}{Problem}
	\newtheorem{proposition}{Proposition}[section]
	\newtheorem{lemma}{Lemma}[section]
	\newtheorem{corollary}[theorem]{Corollary}
	\newtheorem{example}{Example}[section]
	\newtheorem{definition}{Definition}[section]
	%\newtheorem{algorithm}{Algorithm}[section]
	%\newtheorem{cor}{Corollary}
	\newcommand{\BEQA}{\begin{eqnarray}}
		\newcommand{\EEQA}{\end{eqnarray}}
	\newcommand{\define}{\stackrel{\triangle}{=}}
	\newcommand{\myvec}[1]{\ensuremath{\begin{pmatrix}#1\end{pmatrix}}}
	\newcommand{\mydet}[1]{\ensuremath{\begin{vmatrix}#1\end{vmatrix}}}
	
	\bibliographystyle{IEEEtran}
	%\bibliographystyle{ieeetr}
	
	\providecommand{\nCr}[2]{\,^{#1}C_{#2}} % nCr
	\providecommand{\nPr}[2]{\,^{#1}P_{#2}} % nPr
	\providecommand{\mbf}{\mathbf}
	\providecommand{\pr}[1]{\ensuremath{\Pr\left(#1\right)}}
	\providecommand{\qfunc}[1]{\ensuremath{Q\left(#1\right)}}
	\providecommand{\sbrak}[1]{\ensuremath{{}\left[#1\right]}}
	\providecommand{\lsbrak}[1]{\ensuremath{{}\left[#1\right.}}
	\providecommand{\rsbrak}[1]{\ensuremath{{}\left.#1\right]}}
	\providecommand{\brak}[1]{\ensuremath{\left(#1\right)}}
	\providecommand{\lbrak}[1]{\ensuremath{\left(#1\right.}}
	\providecommand{\rbrak}[1]{\ensuremath{\left.#1\right)}}
	\providecommand{\cbrak}[1]{\ensuremath{\left\{#1\right\}}}
	\providecommand{\lcbrak}[1]{\ensuremath{\left\{#1\right.}}
	\providecommand{\rcbrak}[1]{\ensuremath{\left.#1\right\}}}
	\theoremstyle{remark}
	\newtheorem{rem}{Remark}
	\newcommand{\sgn}{\mathop{\mathrm{sgn}}}
	\providecommand{\abs}[1]{\left\vert#1\right\vert}
	\providecommand{\res}[1]{\Res\displaylimits_{#1}} 
	\providecommand{\norm}[1]{\lVert#1\rVert}
	\providecommand{\mtx}[1]{\mathbf{#1}}
	\providecommand{\mean}[1]{E\left[ #1 \right]}
	\providecommand{\fourier}{\overset{\mathcal{F}}{ \rightleftharpoons}}
	\providecommand{\ztrans}{\overset{\mathcal{Z}}{ \rightleftharpoons}}
	
	%\providecommand{\hilbert}{\overset{\mathcal{H}}{ \rightleftharpoons}}
	\providecommand{\system}{\overset{\mathcal{H}}{ \longleftrightarrow}}
	%\newcommand{\solution}[2]{\textbf{Solution:}{#1}}
	\newcommand{\proof}{\noindent \textbf{Proof: }}
	\newcommand{\solution}{\noindent \textbf{Solution: }}
	\providecommand{\dec}[2]{\ensuremath{\overset{#1}{\underset{#2}{\gtrless}}}}
	\numberwithin{equation}{section}
	%\numberwithin{equation}{subsection}
	%\numberwithin{problem}{subsection}
	%\numberwithin{definition}{subsection}
	\makeatletter
	\@addtoreset{figure}{problem}
	\makeatother
	
	\let\StandardTheFigure\thefigure
	%\renewcommand{\thefigure}{\theproblem.\arabic{figure}}
	\renewcommand{\thefigure}{\theproblem}
	
	
	%\numberwithin{figure}{subsection}
	
	\def\putbox#1#2#3{\makebox[0in][l]{\makebox[#1][l]{}\raisebox{\baselineskip}[0in][0in]{\raisebox{#2}[0in][0in]{#3}}}}
	\def\rightbox#1{\makebox[0in][r]{#1}}
	\def\centbox#1{\makebox[0in]{#1}}
	\def\topbox#1{\raisebox{-\baselineskip}[0in][0in]{#1}}
	\def\midbox#1{\raisebox{-0.5\baselineskip}[0in][0in]{#1}}
	
	\vspace{3cm}
	
	\title{ 
		%\logo{
			%}
		Pingala Series
		%	\logo{Octave for Math Computing }
	}
	%\title{
		%	\logo{Matrix Analysis through Octave}{\begin{center}\includegraphics[scale=.24]{tlc}\end{center}}{}{HAMDSP}
		%}
	
	
	% paper title
	% can use linebreaks \\ within to get better formatting as desired
	%\title{Matrix Analysis through Octave}
	%
	%
	% author names and IEEE memberships
	% note positions of commas and nonbreaking spaces ( ~ ) LaTeX will not break
	% a structure at a ~ so this keeps an author's name from being broken across
	% two lines.
	% use \thanks{} to gain access to the first footnote area
	% a separate \thanks must be used for each paragraph as LaTeX2e's \thanks
	% was not built to handle multiple paragraphs
	%
	
	\author{ VIBHAVASU - EP20BTECH11015}
% note the % following the last \IEEEmembership and also \thanks - 
% these prevent an unwanted space from occurring between the last author name
% and the end of the author line. i.e., if you had this:
% 
% \author{....lastname \thanks{...} \thanks{...} }
%                     ^------------^------------^----Do not want these spaces!
%
% a space would be appended to the last name and could cause every name on that
% line to be shifted left slightly. This is one of those "LaTeX things". For
% instance, "\textbf{A} \textbf{B}" will typeset as "A B" not "AB". To get
% "AB" then you have to do: "\textbf{A}\textbf{B}"
% \thanks is no different in this regard, so shield the last } of each \thanks
% that ends a line with a % and do not let a space in before the next \thanks.
% Spaces after \IEEEmembership other than the last one are OK (and needed) as
% you are supposed to have spaces between the names. For what it is worth,
% this is a minor point as most people would not even notice if the said evil
% space somehow managed to creep in.



% The paper headers
%\markboth{Journal of \LaTeX\ Class Files,~Vol.~6, No.~1, January~2007}%
%{Shell \MakeLowercase{\textit{et al.}}: Bare Demo of IEEEtran.cls for Journals}
% The only time the second header will appear is for the odd numbered pages
% after the title page when using the twoside option.
% 
% *** Note that you probably will NOT want to include the author's ***
% *** name in the headers of peer review papers.                   ***
% You can use \ifCLASSOPTIONpeerreview for conditional compilation here if
% you desire.




% If you want to put a publisher's ID mark on the page you can do it like
% this:
%\IEEEpubid{0000--0000/00\$00.00~\copyright~2007 IEEE}
% Remember, if you use this you must call \IEEEpubidadjcol in the second
% column for its text to clear the IEEEpubid mark.



% make the title area
\maketitle

%\newpage

\tableofcontents

%\renewcommand{\thefigure}{\thesection.\theenumi}
%\renewcommand{\thetable}{\thesection.\theenumi}

\renewcommand{\thefigure}{\theenumi}
\renewcommand{\thetable}{\theenumi}

%\renewcommand{\theequation}{\thesection}


\bigskip

\begin{abstract}
This manual provides a simple introduction to Transforms
\end{abstract}
\section{JEE 2019}
Let 
\begin{align}
a_n &= \frac{\alpha^{n}-\beta^{n}}{\alpha - \beta}, \quad n \ge 1
\\
b_n &= a_{n-1} + a_{n+1}, \quad n \ge 2, \quad b_1 =1
\label{eq:10-orig-diff}
\end{align}
Verify the following using a python code.
\begin{enumerate}[label=\thesection.\arabic*
,ref=\thesection.\theenumi]
\item 
\begin{align}
	\sum_{k=1}^{n}a_k = a_{n+2}-1, \quad n \ge 1
\end{align}
\solution
\begin{figure}[!ht]
\includegraphics[width=\columnwidth]{/media/darkwake/VIB2/EE3900/pingala/figs/e1.1.jpg}
\captionof{figure}{}
\label{fig:an21}
\end{figure}
\newline
From \ref{fig:an21} above equation is \textbf{True}
\item 
\begin{align}
	\sum_{k=1}^{\infty}\frac{a_k}{10^k} =\frac{10}{89}
\end{align}
\solution\\
Proposed value of above summation = $\mathbf{\frac{10}{89}}$ = 0.11235955056179775\\
Calculated value from the code = 0.11235955056179774\\
$\therefore$ The above equation is \textbf{True}
\item 
\begin{align}
	b_n =\alpha^n + \beta^n, \quad n \ge 1
\end{align}
\solution
\begin{figure}[!ht]
	\includegraphics[width=\columnwidth]{/media/darkwake/VIB2/EE3900/pingala/figs/e1.3.jpg}
	\captionof{figure}{}
	\label{fig:bn}
\end{figure}
\newline
From \ref{fig:bn} above equation is \textbf{True}
\item 
\begin{align}
	\sum_{k=1}^{\infty}\frac{b_k}{10^k} =\frac{8}{89}
\end{align}
\solution\\
Proposed value of above summation = $\mathbf{\frac{8}{89}}$ = 0.0898876404494382\\
Calculated value from the code = 0.1348314606741573\\
$\therefore$ The above relation is \textbf{False}


\solution\\ The solution to all above questions can be found at:
\begin{lstlisting}
wget https://github.com/DarkWake9/EE3900/blob/main/pingala/codes/e1.py
\end{lstlisting}
\end{enumerate}





\section{Pingala Series}
\begin{enumerate}[label=\thesection.\arabic*,ref=\thesection.\theenumi]
\item The {\em one sided} $Z$-transform of $x(n)$ is defined as 
%\cite{proakis_dsp}
\begin{align}
	X^{+}(z) = \sum_{n = 0}^{\infty}x(n)z^{-n}, \quad z \in \mathbb{C}
	\label{eq:one-Z}
\end{align}


\item The {\em Pingala} series is generated using the difference equation 
\begin{align}
	x(n+2) = x\brak{n+1} + x\brak{n},  \quad x(0) = x(1) = 1, n \ge 0
	\label{eq:1-pingala}
\end{align}
Generate a stem plot for $x(n)$.\\
\solution
\begin{figure}[!ht]
	\includegraphics[width=\columnwidth]{/media/darkwake/VIB2/EE3900/pingala/figs/e2.1.jpg}
	\captionof{figure}{}	\label{fig:bn}
\end{figure}

\item 		Find $X^{+}(z)$.

\solution From \eqref{eq:1-pingala}
\begin{align}
	\mathcal{Z}^+\brak{x(n + 2)} =\\ \mathcal{Z}^+\brak{x(n + 1)} + \mathcal{Z}^+\brak{x(n)} \\
	\implies z^2X^+(z) - z^2x(0) - zx(1)  = \\zX^+(z) - zx(0) + X^+(z)\\
	\brak{z^2 - z - 1}X^+(z) = z^2 \\
	X^+(z) = \frac{1}{1 - z^{-1} - z^{-2}} 
\end{align}
Let, $\alpha$ and $\beta$ be solutions to eqn $z^2 - z - 1 = 0$,
$\implies $they are solutions of  $z^{-2} + z^{-1} - 1 = 0$
\begin{align}
	X^{+}(z)= \frac{1}{\brak{1 - \alpha z^{-1}}\brak{1 - \beta z^{-1}}} \quad |z| > \alpha
	\label{eq:X-z}
\end{align}
%\begin{figure}[!ht]
%	\includegraphics[width=\columnwidth]{/media/darkwake/VIB2/EE3900/pingala/figs/e2.3a.jpg}
%	\captionof{figure}{}
%	\label{fig:xan}
%\end{figure}
%\newline
%From Fig. \ref{fig:xan}: we see that
%\begin{equation}
%		x(n) = a_{n + 1}	\quad	n \geq 1
%		\label{eq:xnan1}
%\end{equation}
\item Find $x(n)$.\\
\solution
Apply $\mathcal{Z}^+$ transform on both sides
\begin{align}
	X^{+}(z) =	\frac{1}{1-z^{-1}-2^{-2}}\\
	=\frac{1}{\left(1-\alpha z^{-1}\right)\left(1-\beta z^{-1}\right)}\\
	=\frac{1}{\alpha-\beta}\left(\frac{\alpha}{1-\alpha z^{-1}}-\frac{\beta}{1-\beta z^{-1}}\right)\\
	=\sum_{n=0}^{\infty} \dfrac{\alpha^{n+1} - \beta^{n+1}}{(\alpha - \beta)}u(n)z^{-n}\\
%	x_n = a_{n+1}	\quad	n \geq 1\\
	\implies x_n = a_{n+1}u(n)
\end{align}
\item Sketch 
\begin{align}
	y(n)	 = x\brak{n-1} + x\brak{n+1},  \quad n \ge 0
	\label{eq:10-orig-diff-rev}
\end{align}
\solution\\
\begin{figure}[!ht]
	\includegraphics[width=\columnwidth]{/media/darkwake/VIB2/EE3900/pingala/figs/e2.5.jpg}
	\captionof{figure}{}
	\label{fig:xan}
\end{figure}
\newline


\item Find $Y^{+}(z)$. \\
\solution\\
\begin{align}
	Y^{+}(z) = \mathcal{Z}^{+}\brak{x(n-1) + x(n+1)}\\
	= z^{-1}(X^{+}(z)) + zX^{+}(z) - zx(0)\\
	= (z + z^{-1})X^{+}(z) - z\\
	= \frac{z + z^{-1}}{1 - z^{-1} - z^{-2}} - z\\
	= \frac{2z^{-1} + 1}{1 - z^{-1} - z^{-2}}
\end{align}
\item Find $y(n)$.\\
\solution From eq \eqref{eq:10-orig-diff-rev}
\begin{align}
	y(n) = (x\brak{n-1} + x\brak{n+1})u(n)\\
	= (a_n + a_{n+2})u(n)
\end{align}
\begin{equation}
\therefore	y(n)= b_{n+1}u(n) = (\alpha^{n+1} + \beta^{n+1})u(n)
\label{eq:yndef}
\end{equation}
\end{enumerate}\section{Power of the Z transform}
\begin{enumerate}[label=\thesection.\arabic*,ref=\thesection.\theenumi]
%problem-3.1
\item Show that 
\begin{align}u(n)
	\sum_{k=1}^{n}a_k = 
	\sum_{k=0}^{n-1}x(n) = x(n)*u(n-1)
\end{align}
\solution %From the eqn \eqref{eq:x-n-def}, we can see that $x(n) = 0\ \forall\ n < 0$,
\begin{align}
	\sum_{k=1}^{n}a_k &= \sum_{k=0}^{n-1}x(k)= \sum_{k = -\infty}^{n - 1}x(k)\\
	&= \sum_{k = -\infty}^{\infty}x(k)u(n - 1 - k) \\
	&= x(n)*u(n - 1)
\end{align}
%problem-3.2
\item Show that 
\begin{align}
	a_{n+2}-1, \quad n \ge 1
\end{align}
can be expressed as 
\begin{align}
	\sbrak{x\brak{n+1}-1}u\brak{n}
\end{align}
\solution %From the eqn \eqref{eq:x-n-def},
\begin{align}
	a_{n+2} - 1 = \sbrak{x(n + 1) - 1}, \quad n \ge 0\\
%\end{align}
%Now, using the definition of $u(n)$,
%\begin{align}
	u(n) = 1 \quad n > 0
\end{align}
\begin{equation}
	\implies a_{n+2} - 1 = \sbrak{x(n + 1) - 1}u(n)
	\label{eq:an2xn}
\end{equation}
%problem-3.3
\item Show that 
\begin{align}
	\sum_{k=1}^{\infty}\frac{a_k}{10^k}= 
	\frac{1}{10}\sum_{k=0}^{\infty}\frac{x\brak{k}}{10^k} =\frac{1}{10}X^{+}\brak{{10}}
\label{eq:x+10}
\end{align}
\solution 
\begin{align}
	\sum_{k=1}^{\infty}\frac{a_k}{10^k} = \frac{1}{10}\sum_{k = 0}^{\infty}\frac{a_{k+1}}{10^k} \\
	= \frac{1}{10}\sum_{k = 0}^{\infty}\frac{x(k)}{10^k} 
	= \frac{1}{10}X^+(10) \\
	= \frac{1}{10}\times\frac{100}{89} = \frac{10}{89}
\end{align}
%problem-3.4
\item Show that 
\begin{align}
	\alpha^n + \beta^n, \quad n \ge 1
	\label{eq:yn-exp}
\end{align}
can be expressed as 
\begin{align}
	w(n) =\brak{\alpha^{n+1} + \beta^{n+1}}u(n)
\end{align}
and find $W(z)$.\\
\solution %Let, $n = k + 1$ in \eqref{eq:yn-exp} and using the definition of $u(n)$, we get: 
\begin{align}
	\alpha^n + \beta^n \quad n \ge 1\\
	\equiv (\alpha^{n+1} + \beta^{n+1})\quad n \ge 0\\
	= (\alpha^{n+1} + \beta^{n+1})u(n)\\
	\intertext{From eq \eqref{eq:yndef}}
	w(n) = \brak{\alpha^{n+1} + \beta^{n+1}}u(n) = y(n)\\
	\therefore W(z) = Y(z) = \frac{1 + 2z^{-1}}{1 - z^{-1} - z^{-2}}
\end{align}

\item Show that 
\begin{align}
	\sum_{k=1}^{\infty}\frac{b_k}{10^k} =
	\frac{1}{10}\sum_{k=0}^{\infty}\frac{y\brak{k}}{10^k} =\frac{1}{10}Y^{+}\brak{{10}}
\label{eq:y+10}
\end{align}
\solution
\begin{align}
	\sum_{k=1}^{\infty}\frac{b_k}{10^k} &= \frac{1}{10}\sum_{k = 0}^{\infty}\frac{b_{k+1}}{10^k} \\
	&= \frac{1}{10}\sum_{k = 0}^{\infty}\frac{y(k)}{10^k} \\
	&= \frac{1}{10}Y^+(z) \\
	&= \frac{1}{10}\times\frac{120}{89} = \frac{12}{89}
\end{align}
\break
%problem-3.6
\item Solve the JEE 2019 problem.\\
\label{pr:1-6}
\solution
\begin{align}
	\sum_{k = 1}^{n}a_k = x(n)*u(n - 1)
\end{align}
also as
\begin{align}
	&x(n)*u(n - 1) \ztrans X(z)z^{-1}U(z) \\
	&= \frac{z^{-1}}{\brak{1 - z^{-1} - z^{-2}}\brak{1 - z^{-1}}} \\
	&= z\sbrak{\frac{1}{1 - z^{-1} - z^{-2}} - \frac{1}{1 - z^{-1}}} \\
	&\ztrans z\sum_{n = 0}^{\infty}\brak{x(n) - 1}z^{-n} \\
	&= \sum_{n = 0}^{\infty}\brak{x(n) - 1}z^{-n + 1} \\
	&= \sum_{n = 0}^{\infty}\brak{x(n + 1) - 1}z^{-n} 
\end{align}
And from \eqref{eq:an2xn}, we get
\begin{equation}
	\sum_{k = 1}^{n}a_k = a_{n+2} - 1
	\label{eq:a2a}
\end{equation}
\end{enumerate}
\onehalfspacing
From \eqref{eq:a2a}, \eqref{eq:x+10}, \eqref{eq:y+10}:\\
Options  a, b, and c are correct\\
Option  d is incorrect

\end{document}